## Derivatives

---

### Ex 1. Derivatives of Functions

---

#### 1)

**Question**

$$
y = \frac{1}{3}x^3 - \frac{3}{2}x^4 + \frac{13}{5}x^5 - 2x^6.
$$

**Solution**

Differentiate term by term:

$$
y' = x^2 - 6x^3 + 13x^4 - 12x^5.
$$

---

#### 2)

**Question**

$$
y = 5x^{15} - x^2 + \frac{1}{3}x - 2.
$$

**Solution**

Differentiate each term:

$$
y' = 75x^{14} - 2x + \frac{1}{3}.
$$

---

#### 3)

**Question**

$$
y = ax^3 + \frac{x}{2} + c.
$$

**Solution**

Constants disappear under differentiation:

$$
y' = 3ax^2 + \frac{1}{2}.
$$

---

#### 4)

**Question**

$$
y = \frac{4}{x^3}.
$$

**Solution**

Rewrite using powers:

$$
y = 4x^{-3}.
$$

Differentiate:

$$
y' = -12x^{-4} = -\frac{12}{x^4}.
$$

---

#### 5)

**Question**

$$
y = 9x^7 + 3x^{-5} - 3x^{-11}.
$$

**Solution**

Differentiate term by term:

$$
y' = 63x^6 - 15x^{-6} + 33x^{-12}.
$$
---

#### 6)

**Question**

$$
y = 3x^{7/3} - 4x^{13/4} + \frac{4}{7}x^{-1/2} + 7^{3/2}.
$$

**Solution**

Differentiate term by term:

$$
\frac{d}{dx}\left(3x^{7/3}\right) = 7x^{4/3},
$$

$$
\frac{d}{dx}\left(-4x^{13/4}\right) = -13x^{9/4},
$$

$$
\frac{d}{dx}\left(\frac{4}{7}x^{-1/2}\right) = -\frac{2}{7}x^{-3/2},
$$

$$
\frac{d}{dx}\left(7^{3/2}\right) = 0.
$$

---

**Final Answer**

$$
y' = 7x^{4/3} - 13x^{9/4} - \frac{2}{7}x^{-3/2}.
$$

---

#### 7)

**Question**

$$
y = \sqrt[3]{x^2}.
$$

**Solution**

Rewrite using powers:

$$
y = x^{2/3}.
$$

Differentiate:

$$
y' = \frac{2}{3}x^{-1/3}.
$$

---

**Final Answer**

$$
y' = \frac{2}{3}x^{-1/3}.
$$

---

#### 8)

**Question**

$$
y = 5\sqrt[3]{x^7}.
$$

**Solution**

Rewrite:

$$
y = 5x^{7/3}.
$$

Differentiate:

$$
y' = \frac{35}{3}x^{4/3}.
$$

---

**Final Answer**

$$
y' = \frac{35}{3}x^{4/3}.
$$

---

#### 9)

**Question**

$$
y = 3\sqrt[3]{x} - x^3 + \frac{2}{3}\sqrt[3]{x^4}.
$$

**Solution**

Rewrite using powers:

$$
y = 3x^{1/3} - x^3 + \frac{2}{3}x^{4/3}.
$$

Differentiate term by term:

$$
y' = x^{-2/3} - 3x^2 + \frac{8}{9}x^{1/3}.
$$

---

**Final Answer**

$$
y' = x^{-2/3} - 3x^2 + \frac{8}{9}x^{1/3}.
$$

---

#### 10)

**Question**

$$
y = \sqrt{x} - 5\sqrt[3]{x^2} - 2\sqrt{x^3}.
$$

**Solution**

Rewrite using powers:

$$
y = x^{1/2} - 5x^{2/3} - 2x^{3/2}.
$$

Differentiate:

$$
y' = \frac{1}{2}x^{-1/2} - \frac{10}{3}x^{-1/3} - 3x^{1/2}.
$$
---

#### 11)

**Question**

$$
y = \frac{2}{\sqrt{z}} - \frac{3}{\sqrt[3]{z}}.
$$

**Solution**

Rewrite using powers:

$$
y = 2z^{-1/2} - 3z^{-1/3}.
$$

Differentiate term by term:

$$
y' = -z^{-3/2} + z^{-4/3}.
$$

---

#### 12)

**Question**

$$
y = \frac{5}{7\sqrt[3]{z}} - 2z^7 + \frac{3}{2\sqrt{z}}.
$$

**Solution**

Rewrite using powers:

$$
y = \frac{5}{7}z^{-1/3} - 2z^7 + \frac{3}{2}z^{-1/2}.
$$

Differentiate:

$$
y' = -\frac{5}{21}z^{-4/3} - 14z^6 - \frac{3}{4}z^{-3/2}.
$$

---

#### 13)

**Question**

$$
x = t^3\sqrt{t}.
$$

**Solution**

Rewrite:

$$
x = t^{3 + 1/2} = t^{7/2}.
$$

Differentiate with respect to $t$:

$$
\frac{dx}{dt} = \frac{7}{2}t^{5/2}.
$$

---

#### 14)

**Question**

$$
y = \frac{2}{z^3\sqrt{z}}.
$$

**Solution**

Rewrite:

$$
y = 2z^{-3}z^{-1/2} = 2z^{-7/2}.
$$

Differentiate:

$$
y' = -7z^{-9/2}.
$$

---

#### 15)

**Question**

$$
y = (2\sqrt[3]{x^2} - x)(4\sqrt[3]{x^4} + 2\sqrt[3]{x^5} + x^2).
$$

**Solution**

Rewrite using powers:

$$
y = (2x^{2/3} - x)(4x^{4/3} + 2x^{5/3} + x^2).
$$

Apply the product rule:

$$
y' = (2x^{2/3} - x)'(4x^{4/3} + 2x^{5/3} + x^2)
$$

$$
\quad + (2x^{2/3} - x)(4x^{4/3} + 2x^{5/3} + x^2)'.
$$

Compute derivatives:

$$
(2x^{2/3} - x)' = \frac{4}{3}x^{-1/3} - 1,
$$

$$
(4x^{4/3} + 2x^{5/3} + x^2)' = \frac{16}{3}x^{1/3} + \frac{10}{3}x^{2/3} + 2x.
$$

---

**Final Answer**

$$
\begin{aligned}
y' =\;&\left(\frac{4}{3}x^{-1/3} - 1\right)
(4x^{4/3} + 2x^{5/3} + x^2)\\
&+ (2x^{2/3} - x)
\left(\frac{16}{3}x^{1/3} + \frac{10}{3}x^{2/3} + 2x\right).
\end{aligned}
$$
---

#### 16)

**Question**

$$
y = (4x^2 - 2x\sqrt{x} + x)(2x + \sqrt{x}).
$$

**Solution**

Rewrite $\sqrt{x}$ as $x^{1/2}$:

$$
y = (4x^2 - 2x^{3/2} + x)(2x + x^{1/2}).
$$

Apply the product rule:

$$
y' = (4x^2 - 2x^{3/2} + x)'(2x + x^{1/2})
+ (4x^2 - 2x^{3/2} + x)(2x + x^{1/2})'.
$$

Compute derivatives:

$$
(4x^2 - 2x^{3/2} + x)' = 8x - 3x^{1/2} + 1,
$$

$$
(2x + x^{1/2})' = 2 + \frac{1}{2}x^{-1/2}.
$$

---

**Final Answer**

$$
\begin{aligned}
y' =\;& (8x - 3x^{1/2} + 1)(2x + x^{1/2}) \\
&+ (4x^2 - 2x^{3/2} + x)\left(2 + \frac{1}{2}x^{-1/2}\right).
\end{aligned}
$$

---

#### 17)

**Question**

$$
y = \frac{3}{3x - 2}.
$$

**Solution**

Rewrite:

$$
y = 3(3x - 2)^{-1}.
$$

Differentiate:

$$
y' = 3(-1)(3x - 2)^{-2}\cdot 3.
$$

---

**Final Answer**

$$
y' = -\frac{9}{(3x - 2)^2}.
$$

---

#### 18)

**Question**

$$
y = \frac{5}{2x^2 - 5x + 1}.
$$

**Solution**

Rewrite:

$$
y = 5(2x^2 - 5x + 1)^{-1}.
$$

Differentiate using the chain rule:

$$
y' = -5(2x^2 - 5x + 1)^{-2}(4x - 5).
$$

---

**Final Answer**

$$
y' = -\frac{5(4x - 5)}{(2x^2 - 5x + 1)^2}.
$$

---

#### 19)

**Question**

$$
y = \frac{3x^2}{7x^2 - x + 2}.
$$

**Solution**

Use the quotient rule:

$$
y' = \frac{(3x^2)'(7x^2 - x + 2) - 3x^2(7x^2 - x + 2)'}{(7x^2 - x + 2)^2}.
$$

Compute derivatives:

$$
(3x^2)' = 6x,
\quad
(7x^2 - x + 2)' = 14x - 1.
$$

---

**Final Answer**

$$
y' =
\frac{6x(7x^2 - x + 2) - 3x^2(14x - 1)}
{(7x^2 - x + 2)^2}.
$$

---

#### 20)

**Question**

$$
y = \frac{8x^3}{x^2 + x - 1}.
$$

**Solution**

Apply the quotient rule:

$$
y' =
\frac{(8x^3)'(x^2 + x - 1) - 8x^3(x^2 + x - 1)'}
{(x^2 + x - 1)^2}.
$$

Compute derivatives:

$$
(8x^3)' = 24x^2,
\quad
(x^2 + x - 1)' = 2x + 1.
$$

---

**Final Answer**

$$
y' =
\frac{24x^2(x^2 + x - 1) - 8x^3(2x + 1)}
{(x^2 + x - 1)^2}.
$$
---

#### 21)

**Question**

$$
y = \frac{z+1}{z-1}.
$$

**Solution**

Apply the quotient rule:

$$
y' =
\frac{(z-1)\cdot 1 - (z+1)\cdot 1}{(z-1)^2}.
$$

Simplify:

$$
y' = \frac{z-1-z-1}{(z-1)^2}
= -\frac{2}{(z-1)^2}.
$$

---

#### 22)

**Question**

$$
y = \frac{5z^2 + z - 2}{z^2 + 7}.
$$

**Solution**

Use the quotient rule:

$$
y' =
\frac{(5z^2 + z - 2)'(z^2 + 7) - (5z^2 + z - 2)(z^2 + 7)'}
{(z^2 + 7)^2}.
$$

Compute derivatives:

$$
(5z^2 + z - 2)' = 10z + 1,
\quad
(z^2 + 7)' = 2z.
$$

---

**Final Answer**

$$
y' =
\frac{(10z+1)(z^2+7) - 2z(5z^2+z-2)}
{(z^2+7)^2}.
$$

---

#### 23)

**Question**

$$
y = \frac{2z - 2x + 3}{z^2 + 2x - 3}.
$$

**Solution**

Differentiate with respect to $z$ (treat $x$ as constant):

$$
y' =
\frac{(2)(z^2 + 2x - 3) - (2z - 2x + 3)(2z)}
{(z^2 + 2x - 3)^2}.
$$

---

**Final Answer**

$$
y' =
\frac{2(z^2 + 2x - 3) - 2z(2z - 2x + 3)}
{(z^2 + 2x - 3)^2}.
$$

---

#### 24)

**Question**

$$
y = \frac{3}{(1 - z^2)(1 - 2z^3)}.
$$

**Solution**

Rewrite:

$$
y = 3(1 - z^2)^{-1}(1 - 2z^3)^{-1}.
$$

Differentiate using the product rule:

$$
y' = 3\Big[
(1 - z^2)^{-1}(1 - 2z^3)'(-1)
+
(1 - 2z^3)^{-1}(1 - z^2)'(-1)
\Big].
$$

Compute derivatives:

$$
(1 - z^2)' = -2z,
\quad
(1 - 2z^3)' = -6z^2.
$$

---

**Final Answer**

$$
y' =
3\left[
\frac{6z^2}{(1-z^2)(1-2z^3)^2}
+
\frac{2z}{(1-z^2)^2(1-2z^3)}
\right].
$$

---

#### 25)

**Question**

$$
y = \frac{\sqrt[3]{z}}{1 - \sqrt[3]{z}}.
$$

**Solution**

Rewrite using powers:

$$
y = \frac{z^{1/3}}{1 - z^{1/3}}.
$$

Apply the quotient rule:

$$
y' =
\frac{\frac{1}{3}z^{-2/3}(1 - z^{1/3}) - z^{1/3}\left(-\frac{1}{3}z^{-2/3}\right)}
{(1 - z^{1/3})^2}.
$$

Simplify numerator:

$$
\frac{1}{3}z^{-2/3}.
$$

---

**Final Answer**

$$
y' =
\frac{1}{3z^{2/3}(1 - z^{1/3})^2}.
$$
---

#### 26)

**Question**

$$
z = \frac{1+\sqrt{t}}{1+\sqrt{z}}.
$$

**Solution**

Treat the denominator as a constant with respect to $t$ and differentiate:

$$
\frac{dz}{dt}
=
\frac{1}{1+\sqrt{z}} \cdot \frac{d}{dt}(1+\sqrt{t}).
$$

Since

$$
\frac{d}{dt}\sqrt{t} = \frac{1}{2\sqrt{t}},
$$

we obtain

---

**Final Answer**

$$
\frac{dz}{dt}
=
\frac{1}{2\sqrt{t}(1+\sqrt{z})}.
$$

---

#### 27)

**Question**

$$
s = (3t + 1)^7.
$$

**Solution**

Apply the chain rule:

$$
\frac{ds}{dt}
=
7(3t+1)^6 \cdot 3.
$$

---

**Final Answer**

$$
\frac{ds}{dt}
=
21(3t+1)^6.
$$

---

#### 28)

**Question**

$$
v = (4z^2 - 5z + 13)^5.
$$

**Solution**

Differentiate using the chain rule:

$$
\frac{dv}{dz}
=
5(4z^2 - 5z + 13)^4 \cdot (8z - 5).
$$

---

**Final Answer**

$$
\frac{dv}{dz}
=
5(8z - 5)(4z^2 - 5z + 13)^4.
$$

---

#### 29)

**Question**

$$
x = \left(\frac{1}{t} + 4\right)^4.
$$

**Solution**

Rewrite:

$$
x = (t^{-1} + 4)^4.
$$

Differentiate:

$$
\frac{dx}{dt}
=
4(t^{-1}+4)^3 \cdot (-t^{-2}).
$$

---

**Final Answer**

$$
\frac{dx}{dt}
=
-4(t^{-1}+4)^3 t^{-2}.
$$

---

#### 30)

**Question**

$$
s = \left(\frac{7t^2 - \frac{1}{2}t + 6}{t}\right)^6.
$$

**Solution**

Let

$$
u = \frac{7t^2 - \frac{1}{2}t + 6}{t}.
$$

Then

$$
s = u^6,
\quad
\frac{ds}{dt} = 6u^5 \frac{du}{dt}.
$$

Simplify $u$:

$$
u = 7t - \frac{1}{2} + \frac{6}{t}.
$$

Differentiate:

$$
\frac{du}{dt} = 7 - \frac{6}{t^2}.
$$

---

**Final Answer**

$$
\frac{ds}{dt}
=
6\left(7t - \frac{1}{2} + \frac{6}{t}\right)^5
\left(7 - \frac{6}{t^2}\right).
$$

---
